Only the TApp case remains for the fundamental lemma

syntax.sig
@@ -5,6 +5,8 @@ Lam : ty -> (tm -> tm) -> tm
 App : tm -> tm -> tm
 TLam : (ty -> tm) -> tm
 TApp : tm -> ty -> tm
+unit : tm
 
 Fun : ty -> ty -> ty
 Forall : (ty -> ty) -> ty
+Unit : ty
